\begin{answer}	
We have:
%
\begin{align}
	p(y = 1|x; \theta, \mu_0, \mu_1, \Sigma)
	&= \frac{p(y =1)p(x|y = 1)}{p(y = 0)p(x|y = 0) + p(y=1)p(x|y = 1)} \\
	&= \frac{1}{1 + \dfrac{p(y = 0)p(x|y = 0)}{p(y=1)p(x|y = 1)}}
\end{align}
%
Let's consider the fraction in the denominator, we have:
%
\begin{align}
	& \dfrac{p(y = 0)p(x|y = 0)}{p(y=1)p(x|y = 1)} \\
	&= \frac{\dfrac{1 - \phi}{(2\pi)^{d/2}|\Sigma|^{1/2}} \exp((x - \mu_1)^T \Sigma^{-1} (x - \mu_1))}{\dfrac{\phi}{(2\pi)^{d/2}|\Sigma|^{1/2}} \exp((x - \mu_0)^T \Sigma^{-1} (x - \mu_0))} \\
	&= \left(\frac{1 - \phi}{\phi}\right) \exp\left( \frac{1}{2} (x - \mu_1)^T \Sigma^{-1} (x - \mu_1) - \frac{1}{2} (x - \mu_0)^T \Sigma^{-1} (x - \mu_0) \right)
\end{align}
% 
Write $x - \mu_1$ as $x - \mu_0 + \mu_0 - \mu_1$ and group similar terms together, the exponent in the above expression (line (12)) can be derived further as follows:
%
\begin{align}
& \frac{1}{2} (x - \mu_1)^T \Sigma^{-1} (x - \mu_0 + \mu_0 - \mu_1) - \frac{1}{2} (x - \mu_0)^T \Sigma^{-1} (x - \mu_0) \\
&= -\frac{1}{2} (\mu_1 - \mu_0)^T \Sigma^{-1} (x - \mu_0) - \frac{1}{2} (\mu_1 - \mu_0)^T \Sigma^{-1} (x - \mu_1) \\
&= -(\mu_1 - \mu_0)^T \Sigma^{-1} (x - \frac{\mu_0 + \mu_1}{2})
\end{align}
%
Putting everything together, we obtain the above fraction equal to:
$$ \exp\left\{-(\mu_1 - \mu_0)^T \Sigma^{-1}x - \left( \log \left( \frac{\phi}{1 - \phi} \right) - \frac{(\mu_1 - \mu_0)^T \Sigma^{-1} (\mu_0 + \mu_1)}{2} \right) \right\} $$
If we let $$\theta = (\mu_1 - \mu_0)^T \Sigma^{-1}x,$$ $$\theta_0 = \log \left( \dfrac{\phi}{1 - \phi} \right) - \dfrac{(\mu_1 - \mu_0)^T \Sigma^{-1} (\mu_0 + \mu_1)}{2},$$ then the posterior probability can be re-written as $\dfrac{1}{1 + \exp(-\theta^T - \theta_0)}$. \\[2pt]
If the threshold to make prediction is $0.5$, the decision boundary will have an equation $\theta^T x + \theta_0 = 0$. \\
\end{answer}
