\begin{answer}
The log-likelihood function of the data is:

\begin{align}
	\ell(\phi, \mu_0, \mu_1, \Sigma)
	&= \log \prod \limits_{i = 1}^{n} p(x^{(i)}|y^{(i)})p(y^{(i)}) \\
	&= \sum \limits_{i = 1}^{n} (\log p(x^{(i)}|y^{(i)}) \log p(y^{(i)})) \\
	&= 
	\begin{aligned}[t]
		& \sum \limits_{i = 1}^{n} \bigg( -\log (2\pi)^{d/2} - \frac{1}{2}\log |\Sigma| - \frac{1}{2}(x^{(i)} - \mu_{y^{(i)}})^T \Sigma^{-1} (x^{(i)} - \mu_{y^{(i)}}) \\
		& + y^{(i)}\log\phi + (1 - y^{(i)})\log(1 - \phi) \bigg)
	\end{aligned}
\end{align}

The maximum likelihood estimate of  $\theta = (\phi, \mu_0, \mu_1, \Sigma)$ are the value which maximizes the log likelihood function. We will solve the equation $\nabla \ell(\theta) = 0$ in order to obtain them. We have:

\begin{align}
	\nabla_{\phi} \ell(\theta) 
	&= \sum \limits_{i = 1}^{n} \left( \frac{y^{(i)}}{\theta} - \frac{1 - y^{(i)}}{1 - \phi} \right)
	= 0
\end{align}

Solve the above equation gives:
$$\hat{\phi} = \frac{1}{n} \sum \limits_{i = 1}^{n} y^{(i)} = \frac{1}{n} \sum \limits_{i = 1}^{n} 1\{y^{(i)} = 1\}$$

Let's consider now:

\begin{align}
	\nabla_{\mu_0} \ell(\theta) &
	= \nabla_{\mu_0} \left( \sum \limits_{i = 1}^{n} - \frac{1}{2} 1\{y^{(i)} = 0\} (x^{(i)} - \mu_0)^T \Sigma^{-1} (x^{(i)} - \mu_0) \right) \\
	&= - \Sigma^{-1} \sum \limits_{i = 1}^{n} 1\{y^{(i)} = 0\}(\mu_0 - x^{i})
\end{align}

Solve the equation $\nabla_{\mu_0} \ell(\theta) = 0$ gives: $$\widehat{\mu_0} = \frac{ \sum_{i = 1}^{n} 1\{y^{(i)} = 0\}x^{(i)}}{\sum_{i = 1}^{n} 1\{y^{(i)} = 0\}}$$
Similarly, we also obtain $$\widehat{\mu_1} = \frac{ \sum_{i = 1}^{n} 1\{y^{(i)} = 1\}x^{(i)}}{\sum_{i = 1}^{n} 1\{y^{(i)} = 1\}}$$ when solving the corresponding equation $\nabla_{\mu_1} \ell(\theta) = 0$.

Lastly, we compute:

\begin{align}
	\nabla_{\Sigma}\ell(\theta) 
	&= \nabla_{\Sigma} \sum \limits_{i = 1}^{n} \left(- \frac{1}{2}\log |\Sigma| - \frac{1}{2}(x^{(i)} - \mu_{y^{(i)}})^T \Sigma^{-1} (x^{(i)} - \mu_{y^{(i)}}) \right) \\
	&= \sum \limits_{i = 1}^{n} \left( -\frac{1}{2} \Sigma^{-1} + \frac{1}{2}  \Sigma^{-1} (x^{(i)} - \mu_{y^{(i)}}) (x^{(i)} - \mu_{y^{(i)}})^T \Sigma^{-1} \right) \\
	&= \frac{1}{2} \Sigma^{-1}\left( \sum \limits_{i = 1}^{n} (x^{(i)} - \mu_{y^{(i)}}) (x^{(i)} - \mu_{y^{(i)}})^T \Sigma^{-1} - n \right)
\end{align}

Solve the equation $\nabla_{\Sigma} \ell(\theta) = 0$, we get:
$$\widehat\Sigma = \frac{1}{n} \sum \limits_{i = 1}^{n} (x^{(i)} - \mu_{y^{(i)}}) (x^{(i)} - \mu_{y^{(i)}})^T$$
In the above derivation of $\nabla_{\Sigma} \ell(\theta)$, we used 2 identities:

\begin{align}
\nabla_{\Sigma}\log|\Sigma| &= (\Sigma^{-1})^T \\
\nabla_{\Sigma} z^T\Sigma^{-1} z &= -\Sigma^{-1} z z^T \Sigma^{-1}, 
\end{align}

where $z$ is not a function of $\Sigma$. To prove the second identity, we take the differential:
\begin{align}
	d(z^T \Sigma^{-1} z) 
	&= d(\text{Tr}[z^T \Sigma^{-1} z]) \\
	&= \text{Tr}[z z^T d\Sigma^{-1}] \\
	&= \text{Tr}[-z z^T \Sigma^{-1} (d\Sigma) \Sigma^{-1}] \\
	&= \text{Tr}[-\Sigma^{-1} z z^T \Sigma^{-1} d\Sigma]
\end{align}
Here, we replace $ d\Sigma^{-1} = -\Sigma^{-1}(d\Sigma)\Sigma^{-1} $ (derived from the identity $\Sigma \Sigma^{-1} = I)$. Thus, $\nabla_{\Sigma} z^T\Sigma^{-1} z = -\Sigma^{-1} z z^T \Sigma^{-1}$. \\
\end{answer}
