\begin{answer}
Consider a single example $x^{(i)}$, we have the objective for this example:
\begin{align}
	\ell_i(W) &= \sum_{j=1}^{d} \log p_s(w_j^T x^{(i)}) + \log|W| \\
	&= \sum_{j=1}^{d} \log\left(\frac{1}{2}\exp(-|w_j^T x^{(i)}|\right) + \log|W| \\
	&= -d\log(2) - \sum_{j=1}^{d}|w_j^T x^{(i)}| + \log|W|
\end{align}
Take its derivative, then:
\begin{align}
	\nabla_W\ell_i(W) &= -\sum_{j=1}^{d}\nabla_W|w_j^T x^{(i)}| + \nabla_W\log|W| \\
	&= -\sum_{j=1}^{d}\sign(w_j^T x^{(i)}) 
	\begin{bmatrix}
		\textbf{0} \\
		{x^{(i)}}^T\text{(row j)} \\
		\textbf{0} \\ 
	\end{bmatrix} 
	+ (W^{-1})^T \\
	&=
	-\begin{bmatrix}
		\sign(w_1^T x^{(i)}) \\
		\vdots \\
		\sign(w_d^T x^{(i)}) \\
	\end{bmatrix}{x^{(i)}}^T + (W^{-1})^T	
\end{align}
Now, we perform the SGA update rule for this example: 
$$W := W + \alpha\left( 
-\begin{bmatrix}
	\sign(w_1^T x^{(i)}) \\
	\vdots \\
	\sign(w_d^T x^{(i)}) \\
\end{bmatrix}{x^{(i)}}^T + (W^{-1})^T \right)$$
\end{answer}
